src/cbor/pulse/raw/everparse/CBOR.Pulse.Raw.EverParse.Test.fst
@@ -7,6 +7,7 @@ open LowParse.Pulse.Base
 open Pulse.Lib.Slice
 module SZ = FStar.SizeT
 
+(*
 ```pulse
 fn test (#pm: perm) (#v: Ghost.erased bytes) (s: slice byte)
   requires pts_to s #pm v ** pure (exists off . validator_success test_parse 0sz v off)
@@ -48,5 +49,30 @@ fn test3 (#pm: perm) (#v: Ghost.erased header) (s: slice byte)
 {
   let x = read_header () s;
   (dfst x).major_type
+}
+```
+*)
+
+open CBOR.Spec.Raw.Format
+open CBOR.Pulse.Raw.Format.Serialize
+module U8 = FStar.UInt8
+
+```pulse
+fn ser
+  (x: cbor_raw)
+  (output: slice U8.t)
+  (#y: Ghost.erased raw_data_item)
+  (#pm: perm)
+requires
+    (exists* v . cbor_match pm x y ** pts_to output v ** pure (Seq.length (serialize_cbor y) <= SZ.v (len output)))
+returns res: SZ.t
+ensures
+    (exists* v . cbor_match pm x y ** pts_to output v ** pure (
+      let s = serialize_cbor y in
+      SZ.v res == Seq.length s /\
+      (exists v' . v `Seq.equal` (s `Seq.append` v'))
+    ))
+{
+  cbor_serialize x output;
 }
 ```
